# **UNIT4. TECHNIQUES OF INTEGRATION**

# **<u>L26. Trigonometric Integrals and Substitution</u>**

$$
\int \sin ^{n} x \cos ^{m} x d x
$$
### Method A. either $n$ or $m$ is odd:

- to use $\sin ^{2} x+\cos ^{2} x=1$ to rewrite the integral

$$
\int \sin ^{3} x \cos ^{2} x d x=\int \sin ^{2} x \cos ^{2} x \sin x d x=\int\left(1-\cos ^{2} x\right) \cos ^{2} x \sin x d x
$$
- Substitution:

$$
\begin{aligned}
&u=\cos x \quad \text { and } \quad d u=-\sin x d x \\
&\int\left(1-\cos ^{2} x\right) \cos ^{2} x \sin x d x=\int\left(1-u^{2}\right) u^{2}(-d u) \\
&=-\frac{1}{3} u^{3}+\frac{1}{5} u^{5}+c=-\frac{1}{3} \cos ^{3} u+\frac{1}{5} \cos ^{5} x+c
\end{aligned}
$$
### Method B. both $m$ and $n$ to be even:

- to use double - angle formulae $\cos ^{2} x=\frac{1+\cos 2 x}{2} ; \quad \sin ^{2} x=\frac{1-\cos 2 x}{2}$
  - $\left(\cos 2 x=\cos ^{2} x-\sin ^{2} x=\cos ^{2} x-\left(1-\cos ^{2} x\right)=2 \cos ^{2} x-1\right)$
  - $(\sin 2 x=2 \sin x \cos x)$
- Keep applying Method B until you can apply Method A (when one of $m$ or $n$ is odd).

$$
\begin{aligned}
&\int \sec ^{n} x \tan ^{m} x d x \\ \\
&\sec ^{2} x=1+\tan ^{2} x \\ \\
&\int \sec ^{2} x d x=\tan x+c \quad \int \sec x \tan x d x=\sec x+c \\ \\
&\int \tan x d x=-\ln (\cos x)+c \quad \int \sec x d x=\ln (\tan x+\sec x)+c \quad\text{(advanced guessing)}
\end{aligned}
$$
### Trigonometric Substitution

(trigonometric integrals turns out to be useful for evaluating integrals involving square roots)

# **<u>L28. Integration by Inverse Substitution; Completing the Square</u>**

| Integral                          | Substitution | Trig identity               |
| --------------------------------- | ------------ | --------------------------- |
| $\int \frac{d x}{\sqrt{x^{2}+1}}$ | $x=\tan u$   | $\tan ^{2} u+1=\sec ^{2} u$ |
| $\int \frac{d x}{\sqrt{x^{2}-1}}$ | $x=\sec u$   | $\sec ^{2} u-1=\tan ^{2} u$ |
| $\int \frac{d x}{\sqrt{1-x^{2}}}$ | $x=\sin u$   | $1-\sin ^{2} u=\cos ^{2} u$ |

### e.g. $\int \frac{d x}{\sqrt{x^{2}+4 x}}$

$v=x+2$ and $d v=d x$

$\rightarrow\quad\int \frac{d x}{\sqrt{(x+2)^{2}-4}}=\int \frac{d v}{\sqrt{v^{2}-4}}$

$v=2 \sec u$ and $d v = 2 \sec u \tan u d u$

$\int \frac{d v}{\sqrt{v^{2}-4}}=\int \frac{2 \sec u \tan u d u}{2 \tan u}=\int \sec u d u=\ln (\sec u+\tan u)+c$

$\sec u=\frac{v}{2} \quad$ and $\quad \tan u=\frac{\sqrt{v^{2}-4}}{2}$

$\int \frac{d x}{\sqrt{(x+2)^{2}-4}}=\ln \left(\frac{v}{2}+\frac{\sqrt{v^{2}-4}}{2}\right)+c$

$=\ln \left(v+\sqrt{v^{2}-4}\right)-\ln 2+c=\ln \left(x+2+\sqrt{x^{2}+4 x}\right)+\tilde{c}$

# <u>**L29. Partial Fractions**</u>

- Definition: rational function as the ratio of two polynomials: $\frac{P(x)}{Q(x)}$

# **<u>L30. Integration by Parts; Reduction Formulae</u>**

### Integration by Parts

$$
(u v)^{\prime}=u^{\prime} v+u v^{\prime} \quad \rightarrow \quad u v^{\prime}=(u v)^{\prime}-u^{\prime} v \quad \rightarrow \quad a v^{\prime} d x=u v-\int u^{\prime} v d x
$$

- e.g.1 $\int \tan ^{-1} x d x$

$$
\begin{aligned}
&\text { with } \quad u=\tan ^{-1} x d x \quad \text { and } \quad v^{\prime}=1 \\
&\text { t.f. } \quad v=x \quad \text { and } \quad u^{\prime}=\frac{1}{1+x^{2}} \\
&\int \tan ^{-1} x d x=\int u v^{\prime} d x=\left(\tan ^{-1} x\right) x-\int \frac{1}{1+x^{2}}(x) d x \\
&=x \tan ^{-1} x-\frac{1}{2} \ln \left|1+x^{2}\right|+c
\end{aligned}
$$

### Alternative Approach to Integration by Parts

$$
\begin{aligned}
&\int_{a}^{b} u v^{\prime} d x=\left.u v\right|_{a} ^{b}-\int_{a}^{b} \\ \\
&\int u d v=u v-\int v d u
\end{aligned}
$$
### Reduction Formulas (Recurrence Formulas)

- e.g.3 $\int(\ln x)^{n} d x$

$$
u=(\ln x)^{n} \rightarrow u^{\prime}=n(\ln x)^{n-1}\left(\frac{1}{x}\right) ; \quad v^{\prime}=d x \rightarrow v=x
$$

$$
\begin{aligned}
&\int(\ln x)^{n} d x=x(\ln x)^{n}-\int n(\ln x)^{n-1} x\left(\frac{1}{x}\right) d x \\
&=x(\ln x)^{n}-n\left(x(\ln x)^{n-1}-\int(n-1)(\ln x)^{n-2} x\left(\frac{1}{x}\right) d x=\ldots\right.
\end{aligned}
$$
### Arc Length

$$
\begin{aligned}
&d s=\sqrt{(d x)^{2}+(d y)^{2}}=\sqrt{1+(d y / d x)^{2}} d x \\
&\int_{P_{0}}^{P_{1}} d s=\int_{a}^{b} \sqrt{1+\left(\frac{d y}{d x}\right)^{2}} d x
\end{aligned}
$$
### Parametric Equations

$$
x=a \cos t ; \quad y=a \sin t ; \quad \rightarrow y^{2}+x^{2}=a^{2}
$$
## **<u>L31. Parametric Equations, Arc Length, Surface Area</u>**

### Arc Length (for Parametric Equations)

### Surface Area (surfaces of revolution)

$$
\text { Area }=\int 2 \pi y d s
$$
# **<u>L32. Polar Co-ordinates, Area in Polar Co-ordinates</u>**

### Polar Co-ordinates

$$
x=r \cos \theta \quad \text { and } \quad y=r \sin \theta
$$
### Area in Polar Coordinates

$$
\text { Area }=\int_{\theta_{1}}^{\theta_{2}} \frac{1}{2} r^{2} d \theta
$$



# **<u>L34. Indeterminate Forms - L'HÃ´pital's Rule</u>**

- when $f(a)=g(a)=0(f(a)=g(a)=\infty$ also works $),\left(g^{\prime}(a) \neq 0\right)$
  $$
  \lim _{x \rightarrow a} \frac{f(x)}{g(x)}=\lim _{x \rightarrow a} \frac{\frac{f(x)}{x-a}}{\frac{g(x)}{x-a}}=\frac{\lim _{x \rightarrow a} \frac{f(x)-f(a)}{x-a}}{\lim _{x \rightarrow a} \frac{g(x)-g(a)}{x-a}}=\frac{f^{\prime}(a)}{g^{\prime}(a)}
  $$

- e.g. $\lim _{x \rightarrow 0} x^{x}$ for $x>0$

$$
\begin{aligned}
&\lim _{x \rightarrow 0} x^{x}=\lim _{x \rightarrow 0} e^{x \ln x} \\
&\lim _{x \rightarrow 0} x \ln x=\lim _{x \rightarrow 0} \frac{\ln x}{1 / x}=\lim _{x \rightarrow 0} \frac{1 / x}{-1 / x^{2}}=0
\end{aligned}
$$
# **<u>L35. Improper Integrals</u>**

### Definition

$$
\int_{a}^{\infty} f(x) d x=\lim _{M \rightarrow \infty} \int_{a}^{M} f(x) d x
$$
- is said to converge if the limit exists (diverges if the limit does not exist).

### Determining Divergence and Convergence

### Improper Integrals of the Second Type

$$
\int_{0}^{1} \frac{d x}{\sqrt{x}}
$$
# **<u>L36. Infinite Series and Convergence Tests</u>**

# **<u>L37. Taylor Series</u>**

$$
\begin{aligned}
&a_{n}=\left(\frac{1}{n !}\right) f^{(n)}(0) \\
&f(x)=\sum_{n=0}^{\infty} \frac{f^{(n)}(0)}{n !} x^{n}
\end{aligned}
$$















